theories/poly/utp_poly_expr.thy
@@ -41,6 +41,11 @@ declare MkPExpr_inverse [simp]
 
 notation DestPExpr ("\<lbrakk>_\<rbrakk>\<^sub>*")
 
+lemma binding_upd_ty_twist [intro]:
+  assumes "e \<rhd>\<^sub>p x" "f \<rhd>\<^sub>p y" "x\<down> \<noteq> y\<down>"
+  shows "b(x :=\<^sub>* e, y :=\<^sub>* f) = b(y :=\<^sub>* f, x :=\<^sub>* e)"
+  using assms by (simp add:binding_upd_ty_def typing binding_upd_twist)
+
 lemma DestPExpr_intro [intro]:
   "(\<And> b. \<lbrakk>x\<rbrakk>\<^sub>*b = \<lbrakk>y\<rbrakk>\<^sub>*b) \<Longrightarrow> x = y"
   by (auto simp add: DestPExpr_inject[THEN sym])
@@ -74,6 +79,14 @@ definition UNREST_PEXPR :: "('m VAR) set \<Rightarrow> ('a, 'm :: VALUE) WF_PEXP
 setup {*
 Adhoc_Overloading.add_variant @{const_name unrest} @{const_name UNREST_PEXPR}
 *}
+
+lemma EvalPE_UNREST_assign [evalp]:
+  "\<lbrakk> v \<rhd>\<^sub>p x; {x\<down>} \<sharp> e \<rbrakk> \<Longrightarrow> \<lbrakk>e\<rbrakk>\<^sub>*(b(x :=\<^sub>* v)) = \<lbrakk>e\<rbrakk>\<^sub>*b"
+  apply (simp add:UNREST_PEXPR_def binding_upd_ty_def)
+  apply (drule_tac x="b" in spec)
+  apply (drule_tac x="b(x\<down> :=\<^sub>b InjU v)" in spec)
+  apply (simp add:typing)
+done
 
 definition LitPE :: "'a \<Rightarrow> ('a :: DEFINED, 'm :: VALUE) WF_PEXPRESSION" where
 "LitPE v = MkPExpr (\<lambda> b. v)"
@@ -1300,12 +1313,14 @@ done
 
 lemma EvalR_AssignR_typed [evalpr]:
   fixes x :: "('a :: DEFINED, 'm :: VALUE) PVAR"
-  assumes "TYPEUSOUND('a, 'm)" "x \<in> PUNDASHED" "e \<rhd>\<^sub>* x" "D\<^sub>1 \<sharp> e"
+  assumes "x \<in> PUNDASHED" "e \<rhd>\<^sub>* x" "D\<^sub>1 \<sharp> e"
   shows "\<lbrakk>x\<down> :=\<^sub>R e\<down>\<rbrakk>R = {(b, b(x:=\<^sub>* (\<lbrakk>e\<rbrakk>\<^sub>* b))) | b. b \<in> WF_REL_BINDING}"
+  using assms
+  apply (subgoal_tac "TYPEUSOUND('a, 'm)")
   apply (subst EvalR_AssignR)
-  apply (simp add:closure assms typing unrest)
+  apply (simp add:closure typing unrest)
   apply (rule PExprE_compat)
-  apply (simp_all add: assms unrest binding_upd_ty_def evale)
+  apply (simp_all add: unrest binding_upd_ty_def evale pevar_compat_TYPEUSOUND)
 done
 
 theorem EvalR_SubstP_UNDASHED_ty [evalr, evalpr] :
